compiler/dsl/coq/ReflexEcho.v
@@ -28,21 +28,30 @@ Definition COMPS (t : COMPT) : comp :=
   | Echo => mk_comp "Echo" "test/echo-00/test.py" []
   end.
 
-Definition INIT : init_prog PAYD COMPT KSTD (init_msg PAYD) IENVD :=
-  [fun s => Spawn _ _ _ _ IENVD Echo None (Logic.eq_refl _)
+Definition NB_CFGD := 1.
+
+Definition CFGD := mk_vvdesc
+  [("Echo", [str_d])
   ].
 
-Definition HANDLERS : handlers PAYD COMPT KSTD :=
+Notation t_cfg_echo := (None) (only parsing).
+
+Definition INIT : init_prog PAYD COMPT KSTD CFGD (init_msg PAYD) IENVD :=
+  [fun s => Spawn _ _ _ CFGD _ IENVD Echo t_cfg_echo
+                  (str_of_string "Echo",tt) None (Logic.eq_refl _)
+  ].
+
+Definition HANDLERS : handlers PAYD COMPT KSTD CFGD :=
   fun (m : msg PAYD) cfd =>
     match m as _m return forall (EQ : _m = m), _ with
     | Build_msg None p => fun EQ =>
       let envd := existT _ 0 tt in
-      existT (fun d => hdlr_prog PAYD COMPT KSTD _ d) envd (
+      existT (fun d => hdlr_prog PAYD COMPT KSTD CFGD _ d) envd (
         let (msg, _) := p in fun st0 =>
-        [ fun s => Send _ _ _ _ _ (CFd PAYD _ _ _) None (mvar EQ None, tt) ]
+        [ fun s => Send _ _ _ _ _ _ (CFd PAYD _ _ _) None (mvar EQ None, tt) ]
       )
     | Build_msg (Some bad) _ =>
       match bad with end
     end (Logic.eq_refl m).
 
-Definition main := mk_main (Build_spec NB_MSG PAYD IENVD KSTD COMPT COMPS INIT HANDLERS).
+Definition main := mk_main (Build_spec NB_MSG PAYD IENVD KSTD COMPT COMPS NB_CFGD CFGD INIT HANDLERS).
