compiler/dsl/coq/ReflexHVec.v
@@ -100,6 +100,32 @@ Implicit Arguments shvec_in [desc n].
 
 Implicit Arguments shvec_replace_ith [desc n].
 
+Fixpoint shvec_match {desc:Set} {n:nat} (vd:svec desc n)
+  (sdenote_desc:desc->Set) (sdenote_desc':desc->Set)
+  (elt_match:forall (d:desc), sdenote_desc d -> sdenote_desc' d -> bool)
+  (v:shvec sdenote_desc vd) (v':shvec sdenote_desc' vd) : bool :=
+  match n as _n
+  return forall (vd' : svec desc _n),
+         shvec sdenote_desc vd' ->
+         shvec sdenote_desc' vd' ->
+         bool
+  with
+  | O => fun _ _ _ => true
+  | S n' => fun vd v v' =>
+    match vd as _vd return
+      @shvec desc sdenote_desc (S n') _vd ->
+      @shvec desc sdenote_desc' (S n') _vd ->
+      bool
+    with
+    | (t, vd') => fun v v' =>
+      match v, v' with
+      | (elt, rest), (elt', rest') =>
+        andb (elt_match t elt elt')
+             (shvec_match vd' sdenote_desc sdenote_desc' elt_match rest rest')
+      end
+    end v v'
+  end vd v v'.
+
 Theorem shvec_ith_in
   (desc : Set) (sdenote_desc : desc -> Set) desc_eqdec
   (UIP_refl_desc : forall (d : desc) (e : d = d), e = Logic.eq_refl d) (n : nat) :
